1. String - a tuple whose every elements is a member of a finite set
2. Prefix - for two strings $y$ and $y'$, we say that $y$ is a prefix of $y'$ if $|y| \le |y'|$ and $y_i = y'_i, \forall i \le |y|$

2. Representation as a String - a representation scheme for any set $\mathcal{O}$ is a pair of functions $(E, D)$ where $E: \mathcal{O} \to \{0,1\}^*$ is a total one-to-one function, $D: \{0,1\}^* \to_{p} \mathcal{O}$ is a possibly partial function and such that $D(E(o)) = o, \forall o \in \mathcal{O}$.
	
	**a) encoding function** - $E$
	- every injective encoding function has a corresponding decoding function - let $E:\mathcal{O} \to \{0,1\}^*$ be one-to-one. Then there exists a function $D:\{0,1\}^* \to \mathcal{O}$ such that $D(E(o)) = o, \forall o \in \mathcal{O}$.
	
	Proof: 
	
	Let $o_0$ be an arbitrary element of $\mathcal{O}$. Since $E$ is one-to-one, then for every $x\in \{0,1\}^*$ there exist either zero or a single $o\in \mathcal{O}$ such that $E(o) = x$. The decoding function can then be defined for those two cases follows:
	
	$$D(x) = \begin{cases} o_0, \text{ when there is no } o\in \mathcal{O} \text{ such that } E(o) = x \\ o, \text{ when there is an } o\in \mathcal{O} \text{ such that } E(o) = x\end{cases}$$
	
	This satisfies the condition that $D$ is onto $\mathcal{O}$.
	
	**b) decoding function** - $D$
	- surjective - $D(E(o)) = o, \forall o\in \mathcal{O}$ means that $D$ must cover the entirety of $O$ because $E$ is a total one-to-one function
	- can technically be partial but is always total for any valid representation scheme due to the proof showing that every one-to-one encoding function has a decoding function
	
	**c) finite representations** - if $\mathcal{O}$ is finite, then every object in it can be represented by a string of length at most $n$, which is in the set $\{0,1\}^{\le n} \coloneqq \{x \in \{0,1\}^*: \vert x\vert \le n\}$
	- encoding function - this needs to be a one-to-one map from $\mathcal{O}$ to $\{0,1\}^{\le n}$, which is only possible if $\vert \mathcal{O} \vert \le \vert \{0,1\}^{\le n} \vert = 2^{n+1} - 1$ due to the pigeonhole principle